\section{Биномиальная формула}
\begin{Def}
$$(((A[x_1])[x_2])[x_3] \ldots )[x_n]$$
кольцо многочленов от n переменных.
$$(A[x_2])[x_1] = (A[x_1])[x_2]$$
$$x_1 \to x_1$$
$$x_2 \to x_2$$

$$\sum c_{i_1, i_2}x_{1}^{i_1}x_2^{i_2}$$
$A[x_1, \ldots, x_n]$ "--- кольцо многочленов от нескольких переменных.
$$\sum c_{i_1, \ldots, i_n}x_1^{i_1}\ldots x_n^{i_n} $$
\end{Def}

{\bf Биномиальная формула:} $(x = y)^n = ?$
{\bf Биномиальные коэффициенты:} $C_n^k = \frac{n!}{k!(n - k)!}$

\begin{lemma} 
\begin{enumerate}
\item $C_n^0 = 1$
\item $C_n^n = 1$
\item $C_n^k + C_n^{k + 1} = C_{n + 1}^{k + 1}$
\item $C_n^{k} = C_{n}^{n - k}$
\end{enumerate}
\end{lemma}
\begin{proof}
$$C_n^k + C_n^{k + 1} = \frac{n!}{k!(n - k)!} + \frac{n!}{(k + 1)!(n - k - 1)!} = $$
$$= \frac{n!(k + 1) + n!(n - k)}{(k + 1)! \ldots (n - k)!} = \frac{n!(n + 1)}{(k + 1)!(n + 1 - (k + 1))!} = C_{n + 1}^{k + 1}$$
\end{proof}

\begin{Def}
\begin{tabular}{c|ccccc}
-&0&1&2&3&4\\
\hline
0&1&-&-&-&-\\
1&1&1&-&-&-\\
2&1&2&1&-&-\\
3&1&3&3&1&-\\
4&1&4&6&4&1\\
\end{tabular}
\end{Def}

\begin{theorem}{Биномиальная формула}
$$(x + y)^k = \sum_{k = 0}^nC_n^kx^ky^{n - k}$$
\end{theorem}

\begin{proof}
Индукция по n
    \begin{enumerate}
        \item n = 0
         $$1 = C^0_0x^0y^0 = 1$$
        \item n = 1
         $$x + y = C_1^0x^1y^0 + C_1^1x^0y^1$$
        \item $n \to n + 1$
        $$(x + y)^{n + 1} = (x + y)^{n}(x + y) = (\sum_{k = 0}^{n}C_n^k)x^ky^{n - k})(x + y) = $$
        $$ = \sum_{k = 0}^{n}C_n^kx^{k + 1}y^{n - k} + \sum_{k = 0}^{n}C_n^kx^ky^{n - k + 1} = $$
        $$ = C_n^nx^{n + 1} + \sum_{k = 0}^{n - 1}C_n^kx^{k + 1}y^{n - k} + \sum_{k = 1}^{n}C_n^kx^ky^{n - k + 1} + C_n^0y^{n + 1} = $$
        $$ = C_{n + 1}^{n + 1}x^{n + 1} + \sum_{k = 1}^{n}C_n^{k - 1}x^{k}y^{n + 1 - k} + \sum_{k = 1}^{n}C_n^kx^ky^{n - k + 1} + C_{n + 1}^0y^{n + 1} = $$
        $$ = C_{n + 1}^{n + 1}x^{n + 1} + \sum_{k = 1}^{n}(C_n^{k - 1} + C_n^{k - 1})x^{k}y^{n + 1 - k} + C_{n + 1}^0y^{n + 1} = $$
        $$ = \sum_{k = 0}^{n + 1}C_{n + 1}^{k}x^{k}y^{n + 1 - k}$$
    \end{enumerate}
\end{proof}

\begin{conseq}
\begin{enumerate}
\item $\sum_{k = 0}^{n}C_n^k = 2^k$
\item $\sum_{k \text{четное}} C_n^k = 2^{n - 1}$
\item $\sum_{k \text{нечетное}} C_n^k = 2^{n - 1}$
\end{enumerate}
\end{conseq}