\section{Производная многочлена}

$A$ - коммутативное кольцо с 1\\
$f \in A[x]$\\
$f = a_nx^n + ... + a_0$\\
$K \in \N, K \cdot a = \underbrace{a + ... + a}_{K раз} = \underbrace{1 + .. + 1}_{K раз}a $ \\
$0 \cdot a = 0$

\begin{Def}
	$f' = n \cdot a_n x^{n-1} + ... + 2a_2x + a_1 = \sum_k = 0^n ka_nx^{k-1}$\\
	($k = 0$ - фиктивное слагаемое, $0 \cdot a_0 x^{-1} = 0$)\\
\end{Def}

\begin{theorem}{}
\textbf{cвойства производной}
	\begin{enumerate}
		\item $(f + g)' = f' + g'$\\
		$f_1 + ... + f_k = f_1' + ... + f_k'$
		\item $c \in A, (c\cdot f)' = c\cdot f'$
		\item $(fg)' = f'g + fg'$
		\item $(f_1 \cdot f_2 \cdot ... \cdot f_k)' = f_1' \cdot f_2 \cdot ... f_k + f_1\cdot f_2'\cdot ... \cdot f_k + ... + f_1 \cdot .. \cdot f_k'$
		\item $A$ - поле, $f \in A[x]$
		\begin{itemize}
			\item $\mathrm{char} A = 0$
				$f' = 0 \Lra f = \mathrm{const}$
			\item $\mathrm{char} A = p > 0$
				$f' = 0 \Lra f \in A[x^p]$
		\end{itemize}
	\end{enumerate}
\end{theorem} 

\begin{proof}
	\begin{enumerate}
		\item упражнение
		\item упражнение
		\item доказываем по частям:
		\begin{itemize}
			\item $f = x^n, g = x^m$\\
				$$(fg)' = (x^{n + m})' = (n + m)x^{n + m -1} = nx^{n-1}x^m + x^n mx^{m-1} = f'g + fg'$$
			\item $f = x^n, g = \sum_{k = 0}^m c_k x^k$\\
				$$(fg)' = (\sum_{k=0}^m c_k x^n x^k)' = \sum_{k=0}^m c_k(x^n x^k)' =$$
				$$ = \sum_{k=0}^m c_k(f'x^k + fkx^{k-1}) = f' \sum_{k=0}^m c_k x^k + f \sum_{k=0}^m kx^{k-1}) = f'g + fg'$$
			\item $f = \sum_{k = 0}^n a_k x^k, g$ - произвольный многочлен\\
				$$ (fg)' = \sum_{k = 0}^n a_k(x^k g)' = \sum_{k = 0}^n a_k(kx^{k-1}g + x^kg') = $$
				$$ = g\sum_{k = 0}^n ka_kx^{k-1} + g'\sum_{k=0}^n a_kx^k = f'g + fg' $$			
		\end{itemize}
		\item упражнение
		\item следствие п.4
		\item 
		\begin{itemize}
			\item $\mathrm{char} A = 0$\\
				$$ f = c_0 + c_1x + ... + c_nx^n$$
				$$ 0 = f' = c_1 + 2c_2x + ... + nc_nx^{n-1} $$
				$$	\forall k, k c_k = 0 \underbrace{(1 + 1 + ... + 1)}_{\neq 0, k раз}c_k = 0 \Ra f = c_0 = \mathrm{const} $$
				\textit{обратное очевидно}
			\item $\mathrm{char} A = p > 0, f' = \sum_{k = 1}^nkc_kx^{k-1}$
				$\forall k \geq 1 kc_k = 0$
		 		Пусть $p \nmid k, k = pq + r, 1 < r <p$
		 		$$ kc_k = \underbrace{(1+1+...+1)}_{k}c_k = (\underbrace{\underbrace{1+...+1}_p+ .. + \underbrace{1+...+1}_p}_q + \underbrace{1+...+1}_r)c_k = \underbrace{(1+..+1)}_{\neq 0, r раз,  т.к. 0 < r < \mathrm{char} A}c_k $$
		 		$$ \Ra c_k = 0$$
		 		$"\La"$ $f = c_0 + c_px^p + c_{2p}x^2p + .. \in A[x^p]$\\
		 		Если $f = \sum_{j = 0}^rc_{jp}x^{jp}$, то $ f' = \sum_{j=0}^r j\underbrace{p}_{= 0, \mathrm{char} A = p}c_{jp}x^{jp-1} = 0 $
		 		
		\end{itemize}	
	\end{enumerate}
\end{proof}
